LinearScan.hs
@@ -1,5 +1,7 @@
 module LinearScan
     ( VirtReg
+    , StartsLoop(..)
+    , EndsLoop(..)
     , ScanState
     , allocateRegisters
     , IntervalId
@@ -9,43 +11,52 @@ module LinearScan
     ) where
 
 import           Control.Applicative
+import           Data.Fin (of_nat_lt)
 import           Data.Fin0
-import           Data.NonEmpty0
 import qualified Data.List.NonEmpty as NE
 import           Data.Main
+import           Data.Maybe
+import           Data.NonEmpty0
 
 type    VirtReg    = Int
 newtype ScanState  = ScanState LinearScan__ScanStateDesc
 newtype PhysReg    = PhysReg { getPhysReg :: LinearScan__PhysReg }
+newtype StartsLoop = StartsLoop { getStartsLoop :: Bool }
+newtype EndsLoop   = EndsLoop { getEndsLoop :: Bool }
 type    IntervalId = Int
 
 toNonEmpty :: NE.NonEmpty a -> NonEmpty a
 toNonEmpty (x NE.:| []) = NE_Sing x
 toNonEmpty (x NE.:| (y:ys)) = NE_Cons x (toNonEmpty (y NE.:| ys))
 
-allocateRegisters
-    :: (block -> Bool)
-    -> (block -> Bool)
-    -> (block -> [Either VirtReg PhysReg])
-    -> NE.NonEmpty block
-    -> ScanState
-allocateRegisters starts ends refs blocks =
-    ScanState (_LinearScan__allocateRegisters
-                   (toNonEmpty (NE.map gather blocks)))
-  where
-    gather b = LinearScan__Build_Block (starts b) (ends b)
-               (map (fmap getPhysReg) (refs b))
+toCoqV :: [a] -> LinearScan__V__Coq_t a
+toCoqV [] = LinearScan__V__Coq_nil
+toCoqV (x:xs) = LinearScan__V__Coq_cons x 0 (toCoqV xs)
 
--- nextInterval :: ScanState -> Int
--- nextInterval (LinearScan__Build_ScanStateDesc ni _ _ _ _ _ _ _) = ni
+-- fromCoqV :: LinearScan__V__Coq_t a -> [a]
+-- fromCoqV LinearScan__V__Coq_nil = []
+-- fromCoqV (LinearScan__V__Coq_cons x _ xs) = x : fromCoqV xs
+
+allocateRegisters
+    :: Int
+    -> (block -> (StartsLoop, EndsLoop, [Either VirtReg PhysReg]))
+    -> NE.NonEmpty block -> ScanState
+allocateRegisters maxVirtReg blockInfo blocks =
+    ScanState $ _LinearScan__allocateRegisters
+        maxVirtReg (toNonEmpty (NE.map gather blocks))
+  where
+    gather b =
+        let (starts, ends, refs) = blockInfo b in
+        LinearScan__Build_Block b (getStartsLoop starts) (getEndsLoop ends) (length refs)
+            (toCoqV (mapMaybe (\x -> case x of
+                                    Left v -> Just (of_nat_lt v maxVirtReg)
+                                    Right _ -> Nothing)
+                     -- (fmap getPhysReg)
+                     refs))
 
 handledIntervalIds :: ScanState -> [IntervalId]
 handledIntervalIds (ScanState (LinearScan__Build_ScanStateDesc ni _ _ _ hnd _ _ _)) =
     map (fin_to_nat ni) hnd
-
--- getInterval :: ScanState -> IntervalId -> Interval
--- getInterval (ScanState (LinearScan__Build_ScanStateDesc ni _ _ _ _ f _ _)) n =
---     Interval (f (from_nat ni n))
 
 registerAssignment :: ScanState -> IntervalId -> Maybe PhysReg
 registerAssignment (ScanState (LinearScan__Build_ScanStateDesc ni _ _ _ _ _ f _)) n =
