Blocks.v
@@ -1,34 +1,164 @@
 Require Import Allocate.
+Require Import Fin.
 Require Import Lib.
+Require Import Machine.
 Require Import NonEmpty.
 Require Import Range.
-Require Import Machine.
+Require Import Vector.
 
+Open Scope nat_scope.
+
+Set Implicit Arguments.
+Unset Strict Implicit.
+Unset Printing Implicit Defensive.
 Generalizable All Variables.
 
 Module MLinearScan (M : Machine).
 Include MAllocate M.
 
+Import EqNotations.
+
 (** * Program graphs *)
 
 Definition VirtReg := nat.
 
-Class Block := {
-    loopStart  : bool;
-    loopEnd    : bool;
-    references : list (VirtReg + PhysReg)
+(** * Block *)
+
+(** An incoming [Block] is really a conceptual "set" of use-positions
+    ([UsePos]), involving several variables and/or registers -- or none (in
+    which case the allocator need not consider it, except to identify the
+    beginning and ending of loops). *)
+
+Section Block.
+
+Variable baseType : Set.
+Variable maxVirtReg : nat.
+
+(* jww (2014-10-18): I do not know how to handle explicit register mentions in
+   the input blocks yet. *)
+(* Definition SomeVar := (fin maxVirtReg + fin maxReg)%type. *)
+Definition SomeVar := (fin maxVirtReg)%type.
+
+Record Block := {
+    original    : baseType;
+    loopBound   : bool;
+    regRequired : bool;
+    refCount    : nat;
+    references  : Vec SomeVar refCount
 }.
 
-Fixpoint processBlocks (maxVirtReg : nat)
-  (blocks : NonEmpty Block) (offset : nat)
-  (start stop : option nat ) : nat * Vec (NonEmpty UsePos) maxVirtReg * nat.
-Admitted.
+Definition boundedRange (pos : nat) :=
+  { rd : RangeDesc | Range rd & pos <= NE_head (ups rd) }.
+
+Definition boundedTriple (pos : nat) :=
+  (option nat * option nat * option (boundedRange pos))%type.
+
+Definition boundedRangeVec (pos : nat) := Vec (boundedTriple pos) maxVirtReg.
+
+Definition boundedTransport (pos : nat) `(Hlt : pos < n)
+  : boundedRangeVec n -> boundedRangeVec pos.
+Proof.
+  rewrite /boundedRangeVec /boundedTriple /boundedRange.
+  elim=> [|[p [[rd r Hr]| ]] n' v' IHv].
+  - by constructor.
+  - constructor; last by apply IHv.
+    split. apply p.
+    apply Some.
+    exists rd. apply r.
+    by abstract ssomega.
+  - constructor; last by apply IHv.
+    split. apply p.
+    by apply None.
+Defined.
+
+Definition boundedSing (upos : UsePos) (Hodd : odd upos) : boundedRange upos.
+Proof. eexists; [ by apply/R_Sing | by [] ]. Defined.
+
+Definition boundedCons (upos : UsePos) (Hodd : odd upos)
+  `(Hlt : upos < n) : boundedRange n -> boundedRange upos.
+Proof.
+  move=> [rd r Hr].
+  eexists; [ by apply/R_Cons => //; apply (ltn_leq_trans Hlt) | by [] ].
+Defined.
+
+Lemma withRanges (pos : nat) (Hodd : odd pos) (req : bool)
+  (upos : UsePos) (Heqe : upos = Build_UsePos pos req)
+  `(Hlt : upos < n) : boundedTriple n -> boundedTriple (uloc upos).
+Proof.
+  move=> [p [[rd r Hr]| ]]; last first.
+    split. by apply p.
+    apply/Some/boundedSing.
+    by rewrite Heqe /=.
+  split. by apply p.
+  apply/Some/(@boundedCons upos).
+  - by rewrite Heqe /=.
+  - by apply n.
+  - by apply Hlt.
+  - by exists rd.
+Defined.
+
+Definition applyList (bs : NonEmpty Block)
+  (base : forall l, boundedRangeVec l.+2)
+  (f : Block -> forall (pos : nat) (Hodd : odd pos),
+         boundedRangeVec pos.+2 -> boundedRangeVec pos)
+   : boundedRangeVec 1 :=
+  let fix go i Hoddi bs :=
+      match bs with
+        | NE_Sing x => f x i Hoddi (base i)
+        | NE_Cons x xs =>
+          f x i Hoddi (go i.+2 (rew <- (odd_succ_succ _) in Hoddi) xs)
+      end in
+  go 1 (RangeTests.odd_1) bs.
+
+Definition emptyBoundedRangeVec (n : nat) : boundedRangeVec n.+2 :=
+  V.const (None, None, None) maxVirtReg.
+
+(** The list of blocks is processed in reverse, so that the resulting
+    sub-lists are also in order. *)
+Definition processBlocks (blocks : NonEmpty Block)
+  : Vec (option RangeSig) maxVirtReg :=
+  let liftOr f mx y :=
+      Some (match mx with Some x => f x y | None => y end) in
+
+  let handle b pos (Hodd : odd pos) (rest : boundedRangeVec pos.+2)
+      : boundedRangeVec pos :=
+      let savingBound x :=
+          if loopBound b
+          then let: (mb, me, r) := x in
+               (liftOr minn mb pos, liftOr maxn me pos, r)
+          else x in
+      let consr (x : boundedTriple pos.+2) : boundedTriple pos :=
+          let upos := Build_UsePos pos (regRequired b) in
+          @withRanges pos Hodd _ upos refl_equal pos.+2 (ltnSSn _) x in
+      let rest' := V.map savingBound rest in
+      match references b with
+      | V.nil => boundedTransport (ltnSSn _) rest'
+      | V.cons v _ vs =>
+        let x := consr (V.nth rest' v) in
+        V.replace (boundedTransport (ltnSSn _) rest') v x
+      (* jww (2014-10-18): See note above. *)
+      (* | V.cons (inr r) _ vs => undefined *)
+      end in
+
+  let res  := applyList blocks emptyBoundedRangeVec handle in
+  V.map (fun x =>
+    let: (mb, me, mr) := x in
+    match mr with
+    | None => None
+    | Some (exist2 rd r _) => Some (exist _ rd r)
+      (* match (mb, me) with *)
+      (* | (None, None) => Some (exist _ rd r) *)
+      (* end *)
+    end) res.
 
 Definition determineIntervals (blocks : NonEmpty Block)
   : { sd : ScanStateDesc | ScanState sd }.
 Admitted.
 
-Definition allocateRegisters (blocks : NonEmpty Block) : ScanStateDesc :=
+Definition allocateRegisters (blocks : NonEmpty Block)
+  : ScanStateDesc :=
   proj1_sig (uncurry_sig linearScan (determineIntervals blocks)).
+
+End Block.
 
 End MLinearScan.
