Vector.v
@@ -18,6 +18,9 @@ Module Import EQ := EqNotations.
 Definition relocate {A n} (v : Vec A n) (p q : fin n) : Vec A n :=
   V.replace v q (V.nth v p).
 
+Definition modify {A n} (v : Vec A n) (p : fin n) (f : A -> A) : Vec A n :=
+  V.replace v p (f (V.nth v p)).
+
 Definition fold_left_with_index {A B : Type} {n} (f : fin n -> B -> A -> B)
   : forall (b : B) (v : Vec A n), B.
   intros b v.
